\noindent \ref{m0:pop:left:emp}  \textbf{event}
\begin{block}
\item \textbf{during}
\begin{block}
\item[ \eqref{m0:pop:left:empdefault} ]$\false $ %
\end{block}
\item \textbf{when}
\begin{block}
\item[ \eqref{m0:pop:left:empm0:grd0} ]$p = q $ %
\end{block}
\item \textbf{begin}
\begin{block}
\item[ \eqref{m0:pop:left:empm0:act0} ]$qe' = qe $ %
\item[ \eqref{m0:pop:left:empm0:act1} ]$p' \1= p $ %
\item[ \eqref{m0:pop:left:empm0:act2} ]$q' = q $ %
\item[ \eqref{m0:pop:left:empm0:act3} ]$res' = res $ %
\item[ \eqref{m0:pop:left:empm0:act4} ]$emp' = (p = q) $ %
\end{block}
\item \textbf{end} \\
\end{block}
